# Appendix A :
## A1:
*first, what is the summation?*

>we can write finite sum of integers  a1, a2, .. an as:

$$\sum_{k=1}^n a_k = a_1 + a_2 + .. + a_n$$
---
### Here some intersting properties of Sumations
\
\
**Linearity**
$$\sum_{k=1}^n (Ca_k + b_k) = C\sum_{k=1}^n a_k + \sum_{k=1}^n b_k .$$

**Arithmetic series**
$$\sum_{k=1}^n k = 1 + 2 + .. + n =   {n(n+1) \ \over 2}$$
$$\sum_{k=0}^n k^2 = 1 + 3 + .. + n^2 =  {n(n+1)(2n+1) \ \over6 }$$
$$\sum_{k=0}^n k^3 = 1 + 8 + .. + n^3 =  {n^2(n+1)^2 \ \over4 }$$

**Geometric series**

$$for\ real\ x\ \  (x \ne 1) :$$

$$\sum_{k=0}^n x^k = 1 + x + .. + x^n =  {x^{n+1} -1  \ \over x^n-1 }$$
for |x|<1
we have infinite decreasing geometric series :





$$\sum_{k=0}^{âˆž} x^k  =  {1  \ \over 1-x }$$

**Harmonic series** for positive integer n, the nth harmonic number is:
$$H_n = 1 + {1 \ \over 2} + {1 \ \over 3} + .. + {1 \ \over n}$$
$$H_n = \sum_{k=1}^n {1 \ \over k} \approx\ ln(n) + O(1)$$
---
---
#### Telscoping series
for any sequance     $a_0 , a_1 , .. a_n :$ *$\sum_{k=1}^n (a_k - a_{k-1}) = a_n - a_0 $*
each element added once and substract once then, similary:
$$\sum_{k=0}^{n-1} (a_{k} - a_{k+1}) = a_0 - a_n$$
an example :
$\sum_{k=1}^{n-1} {1 \ \over k(k+1)} , {1 \ \over k(k+1)}= {1 \ \over k}*{1 \ \over (k+1)}  = {1 \ \over k}-{1 \ \over (k+1)}$
 then,
$$\sum_{k=1}^{n-1} {1 \ \over k}-{1 \ \over (k+1)}$$
$$= 1 - {1 \ \over n}.$$

---
**products**:
$$lg{(\prod_{k=1}^n a_k)}  = \sum_{k=1}^n lg \ a_k$$
>lg is logarithm with base 2 : \
$lg = \log_2$





